Split logrel into more files; clean up relations.v

theories/iris/logrel/fundamental.v
@@ -20,6 +20,7 @@ From Wasm.iris.logrel Require iris_logrel.
 From RichWasm Require Import subst term typing.
 From RichWasm.compiler Require Import codegen instrs modules types util.
 From RichWasm.iris Require Import autowp num_reprs util.
+From RichWasm.iris.logrel Require Import relations util.
 From RichWasm.util Require Import debruijn stdpp_extlib.
 
 Module RT := RichWasm.term.
@@ -29,30 +30,6 @@ Import uPred.
 
 Set Bullet Behavior "Strict Subproofs".
 Set Default Goal Selector "1".
-
-Definition rf : string := "rfN".
-Definition rt : string := "rtN".
-Definition rm : string := "rmN".
-Definition rg : string := "rgN".
-Definition rfN (a : N) : namespace := nroot .@ rf .@ a.
-Definition rtN (a b: N) : namespace := nroot .@ rt .@ a .@ b.
-Definition rmN (a: N) : namespace := nroot .@ rm .@ a.
-Definition rgN (a: N) : namespace := nroot .@ rg .@ a.
-
-Definition rwmem := N.of_nat 0.
-
-Ltac solve_iprop_ne :=
- repeat (apply exist_ne +
-         apply intuitionistically_ne +
-         apply or_ne +
-         apply sep_ne +
-         apply and_ne +
-         apply wp_ne +
-         apply inv_ne +
-         auto +
-         (rewrite /pointwise_relation; intros) +
-         apply forall_ne + apply wand_ne).
-Local Obligation Tactic := try solve_proper.
 
 Ltac fill_vals_pred' vs :=
   instantiate ( 1 := (λ w, ⌜w = vs⌝ ∗ _)%I).
@@ -76,358 +53,12 @@ Ltac fill_vals_pred :=
       fill_vals_pred' vs; iSplitR; [done | fill_goal]
   end.
 
-Definition typ_size (t: value_type) : nat :=
-  match t with
-  | T_i32
-  | T_f32 => 4
-  | T_i64
-  | T_f64 => 8
-  end.
-
-Fixpoint wasm_deser_list (bs: bytes) (vt: list value_type) : list value :=
-  match vt with
-  | vt :: vts =>
-      wasm_deserialise (take (typ_size vt) bs) vt :: wasm_deser_list (drop (typ_size vt) bs) vts
-  | [] => []
-  end.
-
-Definition read_value (τ: RT.Typ) (bs: bytes) : list value :=
-  let vt := translate_type τ in
-  wasm_deser_list bs vt.
-
-Section logrel.
+Section Fundamental.
 
   Context `{!logrel_na_invs Σ}.
   Context `{!wasmG Σ}.
 
   Variable sr : store_runtime.
-
-  Record stack := Stack { stack_values : list value }.
-  Canonical Structure stackO := leibnizO stack.
-
-  Notation VR := ((leibnizO val) -n> iPropO Σ).
-  Notation WR := ((leibnizO value) -n> iPropO Σ).
-  Notation WsR := (stackO -n> iPropO Σ).
-  Notation FR := ((leibnizO frame) -n> iPropO Σ).
-  Notation HR := ((leibnizO bytes) -n> iPropO Σ).
-  Notation ClR := ((leibnizO function_closure) -n> iPropO Σ).
-
-  Definition relations : Type :=
-    (* interp_value *)
-    (leibnizO RT.Typ -n> WsR) *
-    (* interp_frame *)
-    (leibnizO T.Local_Ctx -n> leibnizO wlocal_ctx -n> leibnizO instance -n> FR) *
-    (* interp_expr *)
-    (leibnizO (list RT.Typ) -n>
-     leibnizO T.Function_Ctx -n>
-     leibnizO T.Local_Ctx -n>
-     leibnizO wlocal_ctx -n>
-     leibnizO instance -n>
-     leibnizO (lholed * list administrative_instruction) -n>
-     iPropO Σ).
-
-  Canonical Structure relationsO : ofe := Ofe relations (@prod_ofe_mixin (prodO _ _) _ : OfeMixin relations).
-
-  Program Definition rels_value : relationsO -n> _ :=
-    λne (r: relationsO), r.1.1.
-
-  Program Definition rels_frame : relationsO -n> _ :=
-    λne (r: relationsO), r.1.2.
-
-  Definition rels_expr :
-    relationsO -n>
-    leibnizO (list RT.Typ) -n>
-    leibnizO T.Function_Ctx -n>
-    leibnizO T.Local_Ctx -n>
-    leibnizO wlocal_ctx -n>
-    leibnizO instance -n>
-    leibnizO (lholed * list administrative_instruction) -n>
-    iPropO Σ :=
-    λne (r: relationsO), snd r.
-
-  Global Instance relations_inhabited : Inhabited relationsO.
-  Proof.
-    apply populate.
-    unfold relationsO, relations.
-    exact (λne _ _, ⌜true⌝%I,
-           λne _ _ _ _, ⌜true⌝%I,
-           λne _ _ _ _ _ _, ⌜true⌝%I).
-  Qed.
-
-  Program Definition interp_heap_value_variant : relationsO -n> leibnizO (list RT.Typ) -n> HR :=
-    λne (rs : relationsO) (τs : leibnizO (list RT.Typ)) (bs : leibnizO bytes), (
-      ∃ bs_tag bs_data bs',
-      ⌜bs = bs_tag ++ bs_data ++ bs'⌝ ∗
-      let tagv := wasm_deserialise bs_tag T_i32 in
-      ∃ tag tagi τ,
-      ⌜tagv = VAL_int32 tagi⌝ ∗
-      ⌜nat_repr tag tagi⌝ ∗
-      ⌜τs !! tag = Some τ⌝ ∗
-      let ws := read_value τ bs_data in
-      rels_value rs τ (Stack ws)
-    )%I.
-
-  Program Definition interp_heap_value_struct : relationsO -n> leibnizO (list (RT.Typ * RT.Size)) -n> HR :=
-    λne (rs : relationsO) (fs : leibnizO (list (RT.Typ * RT.Size))) (bs : leibnizO bytes), (
-      ∃ (bss : list bytes) (bs_rest : bytes),
-        ⌜bs = flatten bss ++ bs_rest⌝ ∗
-        [∗ list] f;fbs ∈ fs;bss,
-          let '(τ, sz) := f in
-          let ws := read_value τ fbs in
-          ∃ sz',
-            ⌜sz = SizeConst sz'⌝ ∗
-            ⌜length fbs = (4 * sz')%nat⌝ ∗
-            rels_value rs τ (Stack ws)
-    )%I.
-  Next Obligation.
-    solve_proper_prepare.
-    solve_iprop_ne.
-    apply big_sepL2_ne; intros.
-    destruct y1.
-    solve_iprop_ne.
-    do 4 Morphisms.f_equiv.
-    apply H.
-  Qed.
-
-  Program Definition interp_heap_value_array : relationsO -n> leibnizO RT.Typ -n> HR :=
-    (λne (rs : relationsO) (τ : leibnizO RT.Typ) (bs : leibnizO bytes), ∃ bss bs_rest,
-        (* needs size here *)
-      ⌜bs = flatten bss ++ bs_rest⌝ ∗
-      [∗ list] ebs ∈ bss,
-        let ws := read_value τ ebs in
-        rels_value rs τ (Stack ws))%I.
-  Opaque interp_heap_value_array.
-
-  Definition interp_heap_value : relationsO -> leibnizO RT.HeapType -n> HR :=
-    λ (rs: relationsO), λne (Ψ : leibnizO RT.HeapType),
-    match Ψ with
-    | RT.VariantType τs => interp_heap_value_variant rs τs
-    | RT.StructType fields => interp_heap_value_struct rs fields
-    | RT.ArrayType τ => interp_heap_value_array rs τ
-    | RT.Ex _ _ _ => λne _ , ⌜False⌝%I (* TODO *)
-    end.
-  Instance interp_heap_value_ne : NonExpansive interp_heap_value.
-  Proof.
-    Opaque interp_heap_value_struct.
-    intros n rs rs' Hrs Ψ bs.
-    destruct Ψ; solve_proper.
-    Transparent interp_heap_value_struct.
-  Qed.
-
-  Definition interp_pre_value_unit : WsR := λne ws, ⌜∃ z, head (stack_values ws) = Some (VAL_int32 z)⌝%I.
-
-  Definition interp_values (rs : relations) : leibnizO (list RT.Typ) -n> WsR :=
-    λne (τs : leibnizO (list RT.Typ)) ws, (∃ wss,
-      ⌜stack_values ws = flatten wss⌝ ∗
-      [∗ list] τ;ws ∈ τs;wss, rels_value rs τ (Stack ws)
-    )%I.
-
-  Definition interp_pre_value_num : leibnizO RT.NumType -n> WsR :=
-    λne (np : leibnizO RT.NumType) ws,
-      match np with
-      | RT.Int _ RT.i32 => ⌜∃ z, head (stack_values ws) = Some (VAL_int32 z)⌝%I
-      | RT.Int _ RT.i64 => ⌜∃ z, head (stack_values ws) = Some (VAL_int64 z)⌝%I
-      | RT.Float RT.f32 => ⌜∃ z, head (stack_values ws) = Some (VAL_float32 z)⌝%I
-      | RT.Float RT.f64 => ⌜∃ z, head (stack_values ws) = Some (VAL_float64 z)⌝%I
-      end.
-
-  Definition function_type_args : leibnizO RT.FunType -> leibnizO (seq.seq RT.Typ) :=
-    λ tf,
-      match tf with
-      | RT.FunT _ (Arrow ts _) => ts
-      end.
-  Instance function_type_args_ne :  NonExpansive function_type_args.
-  Proof. solve_proper. Qed.
-
-  Definition function_type_rets : leibnizO RT.FunType -> leibnizO (seq.seq RT.Typ) :=
-    λ tf,
-      match tf with
-      | RT.FunT _ (Arrow _ ts) => ts
-      end.
-  Instance function_type_rets_ne :  NonExpansive function_type_rets.
-  Proof. solve_proper. Qed.
-
-  Definition interp_closure : relationsO -> leibnizO RT.FunType -n> ClR :=
-    λ rs,
-      λne (tf: leibnizO RT.FunType) (cl: leibnizO function_closure),
-      let t1 := function_type_args tf in
-      let t2 := function_type_rets tf in
-      match cl with
-      | FC_func_native inst (Tf wt1 wt2) tlocs es => (<pers> ⌜False⌝)%I
-      | FC_func_host _ _ => ⌜false⌝%I
-      end.
-  Instance interp_closure_rels_ne: NonExpansive (interp_closure) := ltac:(solve_proper).
-
-  Definition interp_pre_value_coderef (rs : relationsO) : leibnizO RT.FunType -n> WsR :=
-    λne tf ws, (
-      ∃ (n : i32) cl,
-      let n' := (Z.to_N (Wasm_int.Int32.unsigned n)) in
-      na_inv logrel_nais (rfN n') (
-        ⌜head (stack_values ws) = Some (VAL_int32 n)⌝ ∗
-        n' ↦[wf] cl ∗
-        ▷ interp_closure rs tf cl
-      )
-    )%I.
-  Instance interp_pre_value_coderef_contractive: Contractive interp_pre_value_coderef :=
-    ltac:(solve_contractive).
-
-  Definition interp_pre_value_exloc (rs : relationsO) : leibnizO RT.Typ -n> WsR :=
-    λne (τ : leibnizO RT.Typ) ws, (∃ ℓ c, ▷ rels_value rs (subst_ext (ext SLoc (LocP ℓ c) id) τ) ws)%I.
-
-  Definition interp_pre_value_ref_own
-    (rs : relationsO)
-  : _ -n> _ -n> _ -n> iPropO Σ :=
-    λne (sz : leibnizO RT.Size) (ψ : leibnizO RT.HeapType) (z : leibnizO i32),
-      ⌜true⌝%I.
-
-  Definition word_aligned (n: N) : Prop :=
-    (4 | n)%N.
-
-  Definition ptr_repr (l: RT.Loc) (i: i32) : Prop :=
-    match l with
-    | RT.LocV v => False
-    | RT.LocP ℓ GCMem =>
-        N_repr (ℓ+1) i /\ word_aligned ℓ
-    | RT.LocP ℓ LinMem =>
-        N_repr ℓ i /\ word_aligned ℓ
-    end.
-
-  Definition interp_value_0 (rs : relations) : leibnizO RT.Typ -n> WsR :=
-    λne (τ: leibnizO RT.Typ), λne vs,
-      let 'Stack vs := vs in
-      match τ with
-      | RT.Num (RT.Int _ RT.i32) => ⌜∃ i, vs = [VAL_int32 i]⌝
-      | RT.Num (RT.Int _ RT.i64) => ⌜∃ i, vs = [VAL_int64 i]⌝
-      | RT.Num (RT.Float RT.f32) => ⌜∃ f, vs = [VAL_float32 f]⌝
-      | RT.Num (RT.Float RT.f64) => ⌜∃ f, vs = [VAL_float64 f]⌝
-      | RT.TVar _ => ⌜False⌝
-      | RT.Unit => ⌜False⌝
-      | RT.ProdT τs => ∃ vss, ⌜vs = flatten vss⌝ ∗ [∗ list] τ;vs ∈ τs;vss, rels_value rs τ (Stack vs)
-      | RT.CoderefT _ => ⌜False⌝
-      | RT.Rec _ _ => ⌜False⌝
-      | RT.PtrT _ => ⌜False⌝
-      | RT.ExLoc _ _ => ⌜False⌝
-      | RT.OwnR _ => ⌜False⌝
-      | RT.CapT _ _ _ => ⌜False⌝
-      | RT.RefT cap (LocP ℓ LinMem) ψ =>
-          ∃ bs l32,
-            ⌜vs = [VAL_int32 l32]⌝ ∗
-            ⌜ptr_repr (LocP ℓ LinMem) l32⌝ ∗
-            N.of_nat sr.(sr_mem_mm) ↦[wms][ℓ] bs ∗
-            interp_heap_value rs ψ bs
-      | RT.RefT _ _ _ => ⌜False⌝
-      end%I.
-
-  Definition interp_frame_0 (rs : relations) : leibnizO T.Local_Ctx -n> leibnizO wlocal_ctx -n> leibnizO instance -n> FR :=
-    (λne (L: leibnizO T.Local_Ctx)
-         (WL: leibnizO wlocal_ctx)
-         (i: leibnizO instance)
-         (f: leibnizO frame),
-       ↪[frame] f ∗
-       ∃ vs wvs: list value,
-           ⌜f = Build_frame (vs ++ wvs) i⌝ ∗
-           (* not right, throws out sizes with (map fst L) *)
-           ▷ interp_values rs (map fst L) (Stack vs) ∗
-           iris_logrel.interp_val WL (immV wvs))%I.
-
-  Program Definition interp_expr_0 (rs : relations) :
-    leibnizO (list RT.Typ) -n>
-    leibnizO T.Function_Ctx -n>
-    leibnizO T.Local_Ctx -n>
-    leibnizO wlocal_ctx -n>
-    leibnizO instance -n>
-    leibnizO (lholed * (seq.seq administrative_instruction)) -n>
-    iPropO Σ :=
-    λne ts C L WL i '(lh, e),
-      (WP e {{ w, ∃ vs, ⌜w = immV vs⌝ ∗
-                        interp_values rs ts (Stack vs) ∗
-                        ∃ f, rels_frame rs L WL i f }})%I.
-
-  Definition rels_0 (rs : relations) : relations :=
-    (interp_value_0 rs,
-     interp_frame_0 rs,
-     interp_expr_0 rs).
-
-  Instance rels_contractive : Contractive rels_0.
-  Proof.
-  Admitted.
-
-  Definition rels : relations := fixpoint rels_0.
-
-  Notation interp_value := (rels_value rels).
-  Notation interp_frame := (rels_frame rels).
-  Notation interp_expr := (rels_expr rels).
-
-  Lemma rels_eq :
-    rels ≡ rels_0 rels.
-  Proof.
-    apply fixpoint_unfold.
-  Qed.
-
-  Lemma interp_value_eq τs vs :
-    interp_value τs vs ⊣⊢ interp_value_0 rels τs vs.
-  Proof.
-    do 2 f_equiv.
-    transitivity (rels_0 rels).1.1.
-    - apply rels_eq.
-    - reflexivity.
-  Qed.
-  Opaque rels_value.
-
-  Lemma interp_expr_eq ts F L WL i e :
-    interp_expr ts F L WL i e ⊣⊢ interp_expr_0 rels ts F L WL i e.
-  Proof.
-    do 6 f_equiv.
-    transitivity (snd (rels_0 rels)).
-    - apply rels_eq.
-    - reflexivity.
-  Qed.
-  Opaque rels_expr.
-
-  Lemma interp_frame_eq L WL i f :
-    interp_frame L WL i f ⊣⊢ interp_frame_0 rels L WL i f.
-  Proof.
-    do 4 f_equiv.
-    transitivity (rels_0 rels).1.2.
-    - apply rels_eq.
-    - reflexivity.
-  Qed.
-  Opaque rels_frame.
-
-  Definition interp_val (τs : list RT.Typ) : VR :=
-    λne (v : leibnizO val), (
-      ⌜v = trapV⌝ ∨ ∃ ws, ⌜v = immV ws⌝ ∗ interp_values rels τs (Stack ws)
-    )%I.
-
-  Definition interp_inst
-    (C: T.Module_Ctx)
-    (inst: instance)
-    : iProp Σ :=
-    ⌜true⌝%I.
-
-  Definition interp_ctx
-    (L L': T.Local_Ctx)
-    (F: T.Function_Ctx)
-    (inst: instance)
-    (lh: lholed)
-    : iProp Σ :=
-    ⌜true⌝%I.
-
-  Definition semantic_typing  :
-    T.Module_Ctx -> T.Function_Ctx ->
-    T.Local_Ctx -> wlocal_ctx ->
-    list administrative_instruction ->
-    RT.ArrowType -> T.Local_Ctx ->
-    iProp Σ :=
-    (λ C F L WL es '(Arrow τs1 τs2) L',
-      ∀ inst lh,
-        interp_inst C inst ∗
-        interp_ctx L L' F inst lh -∗
-        ∀ f vs,
-          interp_val τs1 vs ∗
-          (* frame points to F ∗ *)
-          interp_frame L WL inst f -∗
-          interp_expr τs2 F L' WL inst (lh, (of_val vs ++ es)))%I.
 
   Lemma seq_map_map {A B} (f : A -> B) (l : list A) : seq.map f l = map f l.
   Admitted.
@@ -486,7 +117,7 @@ Section logrel.
     run_codegen (compile_instr me fe
                    (IStructGet (Arrow [RefT cap l hty] [RefT cap l hty; ty], LSig L L) i)) wl =
     inr (tt, wl', es) ->
-    ⊢ semantic_typing M F L [] (to_e_list es) (Arrow [RefT cap l hty] [RefT cap l hty; ty]) L.
+    ⊢ semantic_typing sr M F L [] (to_e_list es) (Arrow [RefT cap l hty] [RefT cap l hty; ty]) L.
   Proof.
     intros -> Htype Hcomp.
     iIntros "%inst %lh [Hinst Hctx] %f %vs [Hval Hfr]".
@@ -501,7 +132,7 @@ Section logrel.
       destruct vss as [|vs vss]; cbn in Hlens; first discriminate Hlens.
       destruct vss; cbn in Hlens; try discriminate Hlens. clear Hlens.
       rewrite big_sepL2_singleton.
-      setoid_rewrite interp_value_eq.
+      setoid_rewrite interp_value_phys_eq.
       cbn.
       setoid_rewrite app_nil_r.
       destruct l; first by iExFalso.
@@ -575,14 +206,14 @@ Section logrel.
   Theorem fundamental_property M F L L' me fe es es' tf wl wl' :
     HasTypeInstrs M F L es tf L' ->
     run_codegen (compile_instrs me fe es) wl = inr (tt, wl', es') ->
-    ⊢ semantic_typing M F L wl' (to_e_list es') tf L'.
+    ⊢ semantic_typing sr M F L wl' (to_e_list es') tf L'.
   Proof.
     intros Htyp Hcomp.
     generalize dependent es'.
     induction Htyp using HasTypeInstrs_mind with (P := fun C F L e ta L' _ =>
       forall es',
       run_codegen (compile_instr me fe e) wl = inr (tt, wl', es') ->
-      ⊢ semantic_typing C F L [] (to_e_list es') ta L');
+      ⊢ semantic_typing sr C F L [] (to_e_list es') ta L');
     intros es' Hcomp.
     - (* INumConst *)
       admit.
@@ -894,7 +525,7 @@ Section logrel.
   Qed.
 
   Lemma read_value_deserialize_i32 sgn b i:
-    read_value (Num (Int sgn RT.i32)) b = [VAL_int32 i] ->
+    deserialize_values b (Num (Int sgn RT.i32)) = [VAL_int32 i] ->
     wasm_deserialise b T_i32 = VAL_int32 i.
   Proof.
   Admitted.
@@ -1015,4 +646,4 @@ Section logrel.
         congruence.
   Qed.
 
-End logrel.
+End Fundamental.
