theories/iris/logrel/util.v
@@ -1,0 +1,40 @@
+From mathcomp Require Import eqtype seq.
+
+Require Import iris.proofmode.tactics.
+
+Require Import RichWasm.term.
+Require Import RichWasm.compiler.types.
+From RichWasm.iris Require Import num_reprs util.
+Import uPred.
+
+Definition wasm_deserialize_values (bs : bytes) (tys : list value_type) : list value :=
+  let bs' := reshape (map length_t tys) bs in
+  zip_with wasm_deserialise bs' tys.
+
+Definition deserialize_values (bs : bytes) : Typ -> list value :=
+  wasm_deserialize_values bs ∘ translate_type.
+
+Definition word_aligned (n : N) : Prop :=
+  (4 | n)%N.
+
+Definition ptr_repr (l : R.Loc) (i : i32) : Prop :=
+  match l with
+  | R.LocV v => False
+  | R.LocP ℓ R.GCMem => N_repr (ℓ + 1) i /\ word_aligned ℓ
+  | R.LocP ℓ R.LinMem => N_repr ℓ i /\ word_aligned ℓ
+  end.
+
+Ltac solve_iprop_ne :=
+  repeat (
+    apply exist_ne +
+    apply intuitionistically_ne +
+    apply or_ne +
+    apply sep_ne +
+    apply and_ne +
+    apply wp_ne +
+    apply inv_ne +
+    auto +
+    (rewrite /pointwise_relation; intros) +
+    apply forall_ne +
+    apply wand_ne
+  ).
